embedded_lemmas.v
@@ -4,7 +4,7 @@ From istari Require Import source subst_src rules_src help subst_help0 subst_hel
      trans basic_types derived_rules.
 From istari Require Import Sigma Tactics
      Syntax Subst SimpSub Promote Hygiene
-     ContextHygiene Equivalence Rules Defined.
+     ContextHygiene Equivalence Equivalences Rules Defined.
 (*useful properties of the embedding*)
 
 Hint Resolve tr_fut_intro: core.
@@ -518,8 +518,12 @@ Lemma leq_trans_app n2 G n1 n3 t1 t2:
 Definition lt_trans_fn_app n1 n2 n3 h12 h23 :=
  (* leq_trans_app (nsucc n1) (nsucc n2) n3
                 (leq_trans_app (nsucc n1) n2 (nsucc n2) h12 (leq_nsucc n2)) (*s(n1) <= s(n2)*)
-                h23.  *) leq_trans_fn_app n1 n2 n3 h12 h23.
+                h23.  *) leq_trans_fn_app (nsucc n1) n2 n3 h12 h23.
 
+(*n1 < n2 (s n1 <= n2)
+ n2 <= n3
+ s n1 <= n3
+ good*)
 Lemma lt_trans_app n2 G n1 n3 t1 t2:
   tr G (oof n1 nattp) ->
   tr G (oof n2 nattp) ->
@@ -528,7 +532,32 @@ Lemma lt_trans_app n2 G n1 n3 t1 t2:
   tr G (oof t2 (leq_t n2 n3)) ->
   tr G (oof (lt_trans_fn_app n1 n2 n3
                           t1 t2)
- (lt_t n1 n3)). Admitted.
+            (lt_t n1 n3)).
+  intros. unfold lt_trans_fn_app. unfold lt_t.
+  unfold lttp. eapply tr_compute.
+  { apply equiv_app. apply reduce_equiv. apply reduce_app_beta;
+                                           apply reduce_id.
+    apply equiv_refl.
+  }
+  {apply equiv_refl. }
+  {apply equiv_refl. }
+  simpsub_bigs. apply leq_trans_app; try apply nsucc_type; try assumption. unfold lt_t in H2. unfold lttp in H2.
+  eapply (tr_compute _ _ (app
+               (app
+                  (lam
+                     (app (subst sh1 leqtp)
+                       (nsucc (var 0)))) n1)
+               n2)).
+  apply equiv_symm.
+  { apply equiv_app. apply reduce_equiv.
+    replace (app leqtp (nsucc n1)) with
+        (subst1 n1 (app leqtp (nsucc (var 0)))).
+    2:{ simpsub_bigs. auto. }
+    apply reduce_app_beta; try apply reduce_id.
+    apply equiv_refl.
+  }
+  {apply equiv_refl. }
+  {apply equiv_refl. } assumption. Qed.
 
 
 Lemma subseq_trans u2 M M' u1 l1 l2 u3 l3 G:
